x86model/REINS/DFACompiler.v
@@ -13,7 +13,6 @@ Require Import ZArith.
 Require Import Bits.
 Require Import PETraversal.
 Require Import ReinsVerifierDFA.
-Require Import ReinsVerifier.
 Require Import Parser.
 Require Import X86Syntax.
 Require Import Decode.
@@ -30,6 +29,7 @@ Open Scope nat_scope.
 Set Printing Depth 10000.
 
 Time Compute (make_dfa reinsjmp_nonIAT_mask).
-Time Compute (make_dfa reinsjmp_IAT_or_RET_mask).
+Time Compute (make_dfa reinsjmp_IAT_JMP_or_RET_mask).
+Time Compute (make_dfa reinsjmp_IAT_CALL_p).
 Time Compute (make_dfa dir_cflow_parser).
 Time Compute (make_dfa non_cflow_parser).
